Too many dependent types.

theories/Coherence/AllocationAlgo.v
@@ -1,15 +1,254 @@
 Require Import CSet Le Arith.Compare_dec.
 
-Require Import Plus Util Map CMap Status Take.
+Require Import Plus Util Map CMap Status Take Filter.
 Require Import Val Var Env IL Annotation Liveness Fresh MoreList SetOperations PairwiseDisjoint.
 Require Import Coherence Allocation RenamedApart MapNotations.
 
 Set Implicit Arguments.
 
+
+Smpl Add
+     match goal with
+     | [ |- @Equivalence.equiv
+             _
+             (@_eq _ (@SOT_as_OT _ (@eq nat) nat_OrderedType))
+             (@OT_Equivalence _ (@SOT_as_OT _ (@eq nat) nat_OrderedType))
+             ?x ?y ] => hnf
+     | [ H : @Equivalence.equiv
+               _
+               (@_eq _ (@SOT_as_OT _ (@eq nat) nat_OrderedType))
+               (@OT_Equivalence _ (@SOT_as_OT _ (@eq nat) nat_OrderedType))
+               ?x ?y |- _ ] => hnf in H; clear_trivial_eqs
+     end : cset.
+
 (** * SSA-based register assignment formulated for IL *)
 
 
-Definition regAssignF
+Definition least_fresh_P (c : var) (G:set var) x :=
+  if [ x <= c ] then least_fresh G else x.
+
+Lemma least_fresh_P_spec c G x
+  : (forall x, x ∈ G -> x <= c)
+    -> least_fresh_P c G x ∉ G.
+Proof.
+  unfold least_fresh_P; cases; eauto using least_fresh_spec.
+Qed.
+
+Lemma filter_add_in X `{OrderedType X} (p:X -> bool) `{Proper _ (_eq ==> eq) p} x s
+  : p x -> filter p {x;s} [=] {x; filter p s}.
+Proof.
+  intros P; split; intros In.
+  - eapply filter_iff in In; eauto.
+    cset_tac. decide (x === a); eauto. right.
+    eapply filter_iff; eauto.
+  - cset_tac; eapply filter_iff; eauto.
+    + cset_tac. rewrite <- H1. eauto.
+    + eapply filter_iff in H1; eauto. cset_tac.
+Qed.
+
+Lemma filter_add_notin X `{OrderedType X} (p:X -> bool) `{Proper _ (_eq ==> eq) p} x s
+  : ~ p x -> filter p {x;s} [=] filter p s.
+Proof.
+  intros P; split; intros In.
+  - eapply filter_iff in In; eauto.
+    cset_tac.
+    + exfalso; eapply P. rewrite H3; eauto.
+    + eapply filter_iff; eauto.
+  - cset_tac; eapply filter_iff; eauto.
+    + eapply filter_iff in In; eauto. cset_tac.
+Qed.
+
+Lemma filter_incl X `{OrderedType X} (p:X -> bool) `{Proper _ (_eq ==> eq) p} s
+  : filter p s ⊆ s.
+Proof.
+  hnf; intros. eapply zfilter_1; eauto.
+Qed.
+
+Lemma filter_add_incl X `{OrderedType X} (p:X -> bool) `{Proper _ (_eq ==> eq) p} s x
+  : filter p {x; s} ⊆ {x; filter p s}.
+Proof.
+  decide (p x).
+  - rewrite filter_add_in; eauto.
+  - rewrite filter_add_notin; eauto with cset.
+Qed.
+
+Lemma lt_minus_lt x y z
+  : x < y - z -> x < y.
+  omega.
+Qed.
+
+Definition crd c (G:set var) (L:list var) :=
+SetInterface.cardinal (filter (fun x0 : nat => if [x0 <= c] then true else false) G) <
+c - SetInterface.cardinal (of_list (List.filter (fun x0 : nat => if [x0 <= c] then true else false) L)).
+
+
+Lemma decons_noext c G x xl
+  : crd c G (x::xl) -> crd c G xl.
+Proof.
+  unfold crd; intros Card. simpl in *. cases in Card; simpl in *.
+  - decide (x ∈ of_list (List.filter (fun x0 : nat => if [x0 <= c] then true else false) xl)).
+    + rewrite add_cardinal_1 in Card. unfold var in *. omega. eauto.
+    + rewrite add_cardinal_2 in Card. unfold var in *. omega. eauto.
+  - eauto.
+Qed.
+
+Lemma decons c G x xl
+      (Card:crd c G (x::xl)) (LE: x <= c) (ND:NoDupA eq (x::xl))
+  : crd c {least_fresh_filter G (lt_minus_lt _ _ Card); G} xl.
+Proof.
+  unfold crd in *; simpl in *.
+  rewrite filter_add_incl, add_cardinal; [| intuition].
+  cases in Card. simpl in *.
+  rewrite add_cardinal_2 in Card. unfold var in *. omega.
+  intro. inv ND.
+  apply of_list_get_first in H; dcr; inv_get. cset_tac.
+  eapply H2.
+  eapply get_InA; eauto.
+Qed.
+
+
+Section FreshListP.
+  Variable c : var.
+
+  Fixpoint fresh_list_P (G:set var) (xl:list var)
+           (LE:crd c G xl) (NoDup:NoDupA eq xl)
+    : list var :=
+    match xl as L return
+          NoDupA eq L -> crd c G L -> list var with
+      | nil => fun _ _ => nil
+      | x::xl => fun ND LE =>
+        match (@decision_procedure (x <= c) _) with
+          | left pf => let y := @least_fresh_filter c G (lt_minus_lt _ _ LE)
+                      in y::@fresh_list_P {y ; G} xl (@decons c G x xl LE pf ND) (NoDupA_decons ND)
+          | right _ => x::@fresh_list_P G xl (@decons_noext c G x xl LE) (NoDupA_decons ND)
+        end
+    end NoDup LE.
+
+
+  Lemma fresh_list_P_length (G:set var) L (LE:crd c G L) (ND:NoDupA eq L)
+  : length (fresh_list_P LE ND) = length L.
+  Proof.
+    general induction L; eauto. simpl fresh_list_P.
+    destruct (@decision_procedure (a <= c) _); simpl.
+    cases; simpl; f_equal; eauto.
+  Qed.
+
+  Lemma fresh_list_P_spec (G:set var) L
+    : (forall x, x > c -> x ∈ of_list L -> x ∈ G -> False)
+      -> NoDupA eq L
+      -> SetInterface.cardinal (filter (fun x => B[x <= c]) G)
+        < c - SetInterface.cardinal (of_list (List.filter (fun x => B[x <= c]) L))
+      -> disj (of_list (fresh_list_P G L)) G.
+  Proof.
+    intros Disj NoDup Card.
+    general induction L; simpl in *; intros; eauto.
+    - hnf; intros. cases in H; simpl in *.
+      + cset_tac.
+        * eapply least_fresh_spec; eauto.
+        * specialize (IHL {least_fresh G; G}).
+          eapply IHL; eauto with cset.
+          -- intros. cset_tac.
+             exploit (least_fresh_small G); eauto.
+             assert (SetInterface.cardinal (filter (fun x : nat => if [x <= c] then true else false) G) <=
+                     SetInterface.cardinal G).
+             rewrite filter_incl; eauto. intuition. unfold var in *. omega.
+          -- rewrite filter_add_incl, add_cardinal.
+             rewrite add_cardinal_2 in Card. unfold var in *. omega.
+             intro. inv NoDup. eapply H4.
+             apply of_list_get_first in H; dcr; inv_get.
+             hnf in H3; subst.
+             eapply get_InA; eauto. clear; intuition.
+      + cset_tac.
+        * eapply (Disj x); eauto. omega.
+        * specialize (IHL G).
+          eapply IHL; eauto with cset.
+  Qed.
+
+   Lemma fresh_list_InA (G: set var) L x
+    : (forall x, x > c -> x ∈ of_list L -> x ∈ G -> False)
+      -> NoDupA eq L
+      -> SetInterface.cardinal G < c - SetInterface.cardinal (of_list (List.filter (fun x => B[x <= c]) L))
+      -> InA eq x (fresh_list_P G L)
+      -> InA eq x L \/ x <= c.
+   Proof.
+     intros. general induction H0; simpl in *.
+     - isabsurd.
+     - cases in H2; simpl in *; invt InA; eauto.
+       + right.
+         rewrite least_fresh_small; eauto. omega.
+       + edestruct (IHNoDupA {least_fresh G; G}); eauto.
+         * intros. eapply H1; cset_tac.
+           exploit (least_fresh_small G); eauto. omega.
+         * rewrite add_cardinal.
+           rewrite add_cardinal_2 in H2; try omega.
+           intro. eapply H.
+           apply of_list_get_first in H4; dcr; inv_get.
+           cset_tac. eapply get_InA; eauto.
+       + edestruct (IHNoDupA G); eauto.
+         * intros. eapply H1; cset_tac.
+   Qed.
+
+  Lemma fresh_list_nodup (G: set var) L
+    : (forall x, x > c -> x ∈ of_list L -> x ∈ G -> False)
+      -> NoDupA eq L
+      -> SetInterface.cardinal G < c - SetInterface.cardinal (of_list (List.filter (fun x => B[x <= c]) L))
+      -> NoDupA eq (fresh_list_P G L).
+  Proof.
+    intros Disj NoDup Card.
+    general induction NoDup; simpl in *; eauto.
+    cases.
+    - econstructor. intro.
+      eapply (@fresh_list_P_spec {least_fresh G; G}); eauto with cset.
+      + intros. cset_tac.
+        exploit (least_fresh_small G); eauto. omega.
+      + rewrite add_cardinal. simpl in *.
+        rewrite add_cardinal_2 in Card.
+        omega.
+        intro. eapply H.
+        apply of_list_get_first in H1; dcr; inv_get.
+        hnf in H3; subst.
+        eapply get_InA; eauto.
+      + eapply InA_in; eauto.
+      + eapply IHNoDup; eauto.
+        * intros. cset_tac.
+          exploit (least_fresh_small G); eauto. omega.
+        * rewrite add_cardinal. simpl in *.
+          rewrite add_cardinal_2 in Card. omega.
+          intro. eapply H.
+          apply of_list_get_first in H0; dcr; inv_get.
+          hnf in H2; subst.
+          eapply get_InA; eauto.
+    - econstructor.
+      + intro. edestruct fresh_list_InA; eauto.
+        cset_tac.
+      + eapply IHNoDup; eauto.
+        intros; cset_tac.
+  Qed.
+End FreshListP.
+
+Lemma least_fresh_P_ext c (G G' : ⦃var⦄) Z
+  : G [=] G' -> least_fresh_P c G Z = least_fresh_P c G' Z.
+Proof.
+  intros. unfold least_fresh_P; cases; eauto.
+  eapply least_fresh_ext; eauto.
+Qed.
+
+Lemma fresh_list_P_ext c (G G' : ⦃var⦄) Z
+  : G [=] G' -> fresh_list_P c G Z = fresh_list_P c G' Z.
+Proof.
+  intros. general induction Z; simpl; eauto.
+  - cases; f_equal; eauto using least_fresh_ext.
+    eapply IHZ. erewrite least_fresh_ext, H; eauto. eauto.
+Qed.
+
+Smpl Add match goal with
+         | [ |- context [ length (fresh_list_P ?c ?G ?Z) ]] =>
+           rewrite (@fresh_list_P_length c G Z)
+         | [ H : context [ length (fresh_list_P ?c ?G ?Z) ] |- _ ] =>
+           rewrite (@fresh_list_P_length c G Z) in H
+         end : len.
+
+Definition regAssignF (c : var)
            (regAssign : stmt -> ann (set var) -> Map [var, var] -> status (Map [var, var]))
   := fix regAssignF
            (ϱ:Map [var, var]) (F:list (list var * stmt)) (ans: list (ann (set var)))
@@ -17,35 +256,34 @@ Definition regAssignF
   match F, ans with
     | Zs::F, a::ans =>
       let Z := fst Zs in let s := snd Zs in
-      let Z' := fresh_list least_fresh (SetConstructs.map (findt ϱ 0) (getAnn a\of_list Z)) (length Z) in
+      let Z' := fresh_list_P c (SetConstructs.map (findt ϱ 0) (getAnn a\of_list Z)) Z in
       sdo ϱ' <- regAssign s a (ϱ[- Z <-- Z'-]);
         regAssignF ϱ' F ans
 
-    | nil, nil => Success ϱ
-    | _, _ => Error "regAssignF: function annotation mismatch"
+    | _, _ => Success ϱ
   end.
 
-Fixpoint regAssign (st:stmt) (an: ann (set var)) (ϱ:Map [var, var])
+Fixpoint regAssign (c : var) (st:stmt) (an: ann (set var)) (ϱ:Map [var, var])
   : status (Map [var, var]) :=
  match st, an with
     | stmtLet x e s, ann1 lv ans =>
-      let xv := least_fresh (SetConstructs.map (findt ϱ 0) (getAnn ans\ singleton x)) in
-        regAssign s ans (ϱ[- x <- xv -])
+      let xv := least_fresh_P c (SetConstructs.map (findt ϱ 0) (getAnn ans\ singleton x)) x
+      in regAssign c s ans ( ϱ[- x <- xv -])
     | stmtIf _ s t, ann2 lv ans ant =>
-      sdo ϱ' <- regAssign s ans ϱ;
-        regAssign t ant ϱ'
+      sdo ϱ' <- regAssign c s ans ϱ;
+        regAssign c t ant ϱ'
     | stmtApp _ _, ann0 _ => Success ϱ
     | stmtReturn _, ann0 _ => Success ϱ
     | stmtFun F t, annF _ ans ant =>
-      sdo ϱ' <- regAssignF regAssign ϱ F ans;
-        regAssign t ant ϱ'
+      sdo ϱ' <- regAssignF c (regAssign c) ϱ F ans;
+        regAssign c t ant ϱ'
     | _, _ => Error "regAssign: Annotation mismatch"
  end.
 
 (** The algorithm only changes bound variables in the mapping [ϱ] *)
 
-Lemma regAssign_renamedApart_agreeF G F ans als ϱ ϱ'
-      (allocOK:regAssignF regAssign ϱ F als = Success ϱ')
+Lemma regAssign_renamedApart_agreeF c G F ans als ϱ ϱ'
+      (allocOK:regAssignF c (regAssign c) ϱ F als = Success ϱ')
       (REN:forall (n : nat) (Zs : params * stmt) (a : ann (set var * set var)),
              get F n Zs -> get ans n a -> renamedApart (snd Zs) a)
       (LEN1:length F = length als)
@@ -56,7 +294,7 @@ Lemma regAssign_renamedApart_agreeF G F ans als ϱ ϱ'
              forall (al : ann (set var * set var)) (ϱ0 ϱ'0 : Map  [var, var])
                (G0 : set var),
                renamedApart (snd Zs) al ->
-               regAssign (snd Zs) a ϱ0 = Success ϱ'0 ->
+               regAssign c (snd Zs) a ϱ0 = Success ϱ'0 ->
                agree_on eq (G0 \ snd (getAnn al)) (findt ϱ0 0) (findt ϱ'0 0)))
 : forall G' : set var,
     list_union zip defVars F ans[<=]G' ->
@@ -65,21 +303,21 @@ Proof.
  intros G' INCL.
  length_equify. general induction LEN1; inv LEN2; simpl in * |- *; try monadS_inv allocOK; eauto.
  exploit IHLEN1; eauto using get.
- etransitivity; try eapply INCL.
- norm_lunion. eauto with cset.
- exploit IH; eauto using get.
- (rewrite <- map_update_list_update_agree in H0; eauto).
- etransitivity; try eapply H.
- eapply agree_on_incl.
- eapply update_with_list_agree_inv; try eapply X; eauto.
- instantiate (1:=G). rewrite minus_union.
- eapply incl_minus_lr; eauto.
- erewrite <- INCL. norm_lunion. unfold defVars. eauto with cset.
+ - etransitivity; try eapply INCL.
+   norm_lunion. eauto with cset.
+ - exploit IH; eauto using get.
+   (rewrite <- map_update_list_update_agree in H0; eauto with len).
+   etransitivity; try eapply H.
+   eapply agree_on_incl.
+   eapply update_with_list_agree_inv; try eapply H0; eauto with len.
+   instantiate (1:=G). rewrite minus_union.
+   eapply incl_minus_lr; eauto.
+   erewrite <- INCL. norm_lunion. unfold defVars. eauto with cset.
 Qed.
 
 
-Lemma regAssign_renamedApart_agree' i s al ϱ ϱ' ZL Lv alv G
-      (allocOK:regAssign s alv ϱ = Success ϱ')
+Lemma regAssign_renamedApart_agree' c i s al ϱ ϱ' ZL Lv alv G
+      (allocOK:regAssign c s alv ϱ = Success ϱ')
       (sd:renamedApart s al)
       (LS:live_sound i ZL Lv s alv)
 : agree_on eq (G \ snd (getAnn al)) (findt ϱ 0) (findt ϱ' 0).
@@ -107,10 +345,10 @@ Proof.
     eapply incl_minus_lr; try reflexivity. rewrite <- H13. eauto with cset.
 Qed.
 
-Lemma regAssign_renamedApart_agree i s al ϱ ϱ' ZL Lv alv
+Lemma regAssign_renamedApart_agree c i s al ϱ ϱ' ZL Lv alv
       (sd:renamedApart s al)
       (LS:live_sound i ZL Lv s alv)
-      (allocOK:regAssign s alv ϱ = Success ϱ')
+      (allocOK:regAssign c s alv ϱ = Success ϱ')
 : agree_on eq (fst (getAnn al)) (findt ϱ 0) (findt ϱ' 0).
 Proof.
   eapply agree_on_incl.
@@ -121,8 +359,8 @@ Proof.
   clear_all; cset_tac; intuition; eauto.
 Qed.
 
-Lemma regAssignF_get G F ans alv n Zs a ϱ ϱ' an ZL Lv i D Dt lv
-: regAssignF regAssign ϱ F alv = Success ϱ'
+Lemma regAssignF_get c G F ans alv n Zs a ϱ ϱ' an ZL Lv i D Dt lv
+: regAssignF c (regAssign c) ϱ F alv = Success ϱ'
   -> (forall n Zs a, get F n Zs -> get ans n a -> renamedApart (snd Zs) a)
   -> (forall n Zs a, get F n Zs ->
                get alv n a ->
@@ -138,34 +376,35 @@ Lemma regAssignF_get G F ans alv n Zs a ϱ ϱ' an ZL Lv i D Dt lv
   -> get alv n a
   -> get ans n an
   -> lv ⊆ D
-  -> exists ϱ1 ϱ2, regAssign (snd Zs) a ϱ1 = Success ϱ2
-             /\ regAssignF regAssign ϱ2 (drop (S n) F) (drop (S n) alv) = Success ϱ'
+  -> exists ϱ1 ϱ2, regAssign c (snd Zs) a ϱ1 = Success ϱ2
+             /\ regAssignF c (regAssign c) ϱ2 (drop (S n) F) (drop (S n) alv) = Success ϱ'
              /\ agree_on eq (G \ list_union (zip defVars (take n F) (take n ans)))
-                        (findt (ϱ[-fst Zs <-- fresh_list least_fresh
+                        (findt (ϱ[-fst Zs <-- fresh_list_P c
                                       (SetConstructs.map (findt ϱ 0) (getAnn a \ of_list (fst Zs)))
-                                      (length (fst Zs))-]) 0)
+                                      (fst Zs)-]) 0)
                         (findt ϱ1 0).
+
 Proof.
   intros EQ REN LV LVINC DDISJ FUNC PWDISJ GET1 GET2 GET3 incl.
   general induction GET1; inv GET2; inv GET3; simpl in * |- *; monadS_inv EQ; eauto.
   - do 2 eexists; split; eauto. split. rewrite EQ0. reflexivity. reflexivity.
-  - exploit (IHGET1 G); hnf; intros; eauto using get; dcr.
+  - exploit (IHGET1 c G); hnf; intros; eauto using get; dcr.
     do 2 eexists; split; eauto. split; eauto.
     rewrite EQ0. simpl. rewrite EQ1; eauto.
     etransitivity; eapply agree_on_incl; [ | reflexivity | eassumption | eauto ].
-    + repeat rewrite <- map_update_list_update_agree; eauto.
-      erewrite least_fresh_list_ext; eauto.
-      * eapply update_with_list_agree; eauto.
+    + repeat rewrite <- map_update_list_update_agree; eauto with len.
+      erewrite fresh_list_P_ext; eauto.
+      * eapply update_with_list_agree; eauto with len.
         eapply regAssign_renamedApart_agree' in EQ0; eauto using get.
-        rewrite <- map_update_list_update_agree in EQ0; eauto.
-        eapply update_with_list_agree_inv in EQ0; eauto.
+        rewrite <- map_update_list_update_agree in EQ0; eauto with len.
+        eapply update_with_list_agree_inv in EQ0; eauto with len.
         eapply agree_on_incl. eauto.
         instantiate (1:=G \ list_union zip defVars (take n xl) (take n xl1)).
         norm_lunion. unfold defVars at 1. clear_all; cset_tac; intuition.
       * eapply lookup_set_agree; eauto.
         eapply regAssign_renamedApart_agree' in EQ0; eauto using get.
-        rewrite <- map_update_list_update_agree in EQ0; eauto.
-        eapply update_with_list_agree_inv in EQ0; eauto.
+        rewrite <- map_update_list_update_agree in EQ0; eauto with len.
+        eapply update_with_list_agree_inv in EQ0; eauto with len.
         eapply agree_on_incl; eauto.
         instantiate (1:=getAnn a \ of_list (fst x)).
         setoid_rewrite minus_union at 1.
